Gt3/SubTy/Cmp.lean
@@ -1,0 +1,5 @@
+-- import Gt3.SubTy.Basic
+
+-- theorem Ctx.JEq.cmp_of_common {Γ A B a b c} (hab : JEq Γ A a b) (hbc : JEq Γ B b c) : CmpTy Γ A B
+--   := by induction hab generalizing B c with
+--   | _ => sorry
